lakefile.lean
@@ -9,3 +9,7 @@ require mathlib from git
 @[default_target]
 lean_lib SSBX where
   srcDir := "formal"
+
+lean_exe «wenyan-surface» where
+  root := `WenyanSurface
+  supportInterpreter := true
